work on flush

lib/Buckets/BucketModel.i.dfy
@@ -11,8 +11,9 @@ include "../../PivotBetree/Bounds.i.dfy"
 module BucketModel {
   import opened BucketsLib
   import opened BucketWeights
-  import PivotsLib
+  import opened PivotsLib
   import opened Lexicographic_Byte_Order
+  import Keyspace = Lexicographic_Byte_Order
   import opened ValueMessage
   import opened Maps
   import opened Sequences
@@ -24,27 +25,133 @@ module BucketModel {
   import opened NativeTypes
   
   datatype singleMergeResult =
-      MergeCompleted(bot: Bucket, slack: uint64)
-    | SlackExhausted(bot: Bucket, end: uint64, slack: uint64)
-
-  function mergeToOneChild(top: Bucket, from: nat, to: nat, bot: Bucket, slack: nat) : (result: singleMergeResult)
-    requires WFBucket(top)
-    requires BucketWellMarshalled(top)
-    requires from <= to < |top.keys|
-    requires WFBucket(bot)
-    requires BucketWellMarshalled(bot)
+    | MergeCompleted(
+        keys: seq<Key>,
+        msgs: seq<Message>,
+        slack: nat)
+    | SlackExhausted(
+        keys: seq<Key>,
+        msgs: seq<Message>,
+        end: nat,
+        slack: nat)
   {
-    assume false;
-    MergeCompleted(bot, 0)
+    function bucketMap() : BucketMap
+    requires |this.keys| == |this.msgs|
+    {
+      BucketMapOfSeq(this.keys, this.msgs)
+    }
+
+    function flushedKeys(
+      top_keys: seq<Key>,
+      top_msgs: seq<Message>,
+      from: nat,
+      to: nat) : set<Key>
+    requires 0 <= from <= to <= |top_keys| == |top_msgs|
+    requires this.SlackExhausted? ==> from <= this.end <= |top_keys|
+    {
+      if this.MergeCompleted? then
+        set key | key in top_keys[from..to]
+      else
+        set key | key in top_keys[from..this.end]
+    }
+
+    function flushedMap(
+      top_keys: seq<Key>,
+      top_msgs: seq<Message>,
+      from: nat,
+      to: nat) : BucketMap
+    requires 0 <= from <= to <= |top_keys| == |top_msgs|
+    requires this.SlackExhausted? ==> from <= this.end <= |top_keys|
+    {
+      var top := BucketMapOfSeq(
+            top_keys[from..to], top_msgs[from..to]);
+      map key | key in top
+        && key in this.flushedKeys(top_keys, top_msgs, from, to)
+        :: top[key]
+    }
   }
-    
+
+  function mergeToOneChild(
+      top_keys: seq<Key>,
+      top_msgs: seq<Message>,
+      from: nat,
+      to: nat,
+      bot_keys: seq<Key>,
+      bot_msgs: seq<Message>,
+      bot_from: nat,
+      acc_keys: seq<Key>,
+      acc_msgs: seq<Message>,
+      slack: nat
+    ) : (result: singleMergeResult)
+  requires |top_keys| == |top_msgs|
+  requires |bot_keys| == |bot_msgs|
+  requires |acc_keys| == |acc_msgs|
+  requires from <= to <= |top_keys|
+  requires bot_from <= |bot_keys|
+  decreases |top_keys| + |bot_keys| - from - bot_from
+  ensures |result.keys| == |result.msgs|
+  ensures result.SlackExhausted? ==> from <= result.end <= |top_keys|
+  {
+    if from == to then
+      MergeCompleted(
+        acc_keys + bot_keys[bot_from..],
+        acc_msgs + bot_msgs[bot_from..],
+        slack)
+    else if |bot_keys| == bot_from then
+      MergeCompleted(
+        acc_keys + top_keys[from..to],
+        acc_msgs + top_msgs[from..to],
+        slack)
+    else if top_keys[from] == bot_keys[bot_from] then
+      var key := top_keys[from];
+      var topmsg := top_msgs[from];
+      var botmsg := bot_msgs[bot_from];
+      var msg := ValueMessage.Merge(topmsg, botmsg);
+      if msg == IdentityMessage() then
+        mergeToOneChild(
+            top_keys, top_msgs, from+1, to,
+            bot_keys, bot_msgs, bot_from+1,
+            acc_keys, acc_msgs,
+            slack + WeightKey(key) + WeightMessage(botmsg))
+      else (
+        var delta := WeightMessage(msg) - WeightMessage(botmsg);
+        if delta > slack then
+          SlackExhausted(acc_keys+bot_keys[bot_from..], acc_msgs+bot_msgs[bot_from..], from, slack)
+        else
+          mergeToOneChild(
+              top_keys, top_msgs, from+1, to,
+              bot_keys, bot_msgs, bot_from+1,
+              acc_keys + [key], acc_msgs + [msg],
+              slack - delta)
+      )
+    else if Keyspace.lt(top_keys[from], bot_keys[bot_from]) then
+      var key := top_keys[from];
+      var msg := top_msgs[from];
+      var delta := WeightKey(key) + WeightMessage(msg);
+      if delta > slack then
+        SlackExhausted(acc_keys+bot_keys[bot_from..], acc_msgs+bot_msgs[bot_from..], from, slack)
+      else
+        mergeToOneChild(
+            top_keys, top_msgs, from+1, to,
+            bot_keys, bot_msgs, bot_from,
+            acc_keys + [key], acc_msgs + [msg],
+            slack - delta)
+    else
+      var key := bot_keys[bot_from];
+      var msg := bot_msgs[bot_from];
+      mergeToOneChild(
+          top_keys, top_msgs, from, to,
+          bot_keys, bot_msgs, bot_from+1,
+          acc_keys + [key], acc_msgs + [msg],
+          slack)
+  }
 
   datatype partialFlushResult = partialFlushResult(
     newParent: Bucket,
     newChildren: seq<Bucket>,
     flushedKeys: set<Key>)
 
-  function {:opaque} partialFlush(parent: Bucket, children: seq<Bucket>, pivots: seq<Key>) : (res: partialFlushResult)
+  /*function {:opaque} partialFlush(parent: Bucket, children: seq<Bucket>, pivots: seq<Key>) : (res: partialFlushResult)
     requires WFBucket(parent)
     requires PivotsLib.WFPivots(pivots)
     requires |pivots| + 1 == |children|
@@ -61,5 +168,595 @@ module BucketModel {
   {
     assume false;
     partialFlushResult(parent, [], {}) // FIXME
+  }*/
+
+  function topBotAccMergeForKey(
+    top: BucketMap,
+    bot: BucketMap,
+    acc: BucketMap,
+    key: Key) : Message
+  {
+    var topmsg := if key in top then top[key] else IdentityMessage();
+    var botmsg := if key in acc then acc[key] else
+        if key in bot then bot[key] else IdentityMessage();
+    ValueMessage.Merge(topmsg, botmsg)
   }
+
+  function topBotAccMerge(
+    top: BucketMap,
+    bot: BucketMap,
+    acc: BucketMap) : BucketMap
+  {
+    map key | key in top.Keys + bot.Keys + acc.Keys
+      && topBotAccMergeForKey(top, bot, acc, key) != IdentityMessage()
+      :: topBotAccMergeForKey(top, bot, acc, key)
+  }
+
+  lemma BucketMapOfSeqPushBack(
+      keys: seq<Key>, msgs: seq<Message>, key: Key, msg: Message)
+  requires |keys| == |msgs|
+  requires IsStrictlySorted(keys)
+  requires forall k | k in keys :: Keyspace.lt(k, key)
+  ensures BucketMapOfSeq(keys + [key], msgs + [msg])
+       == BucketMapOfSeq(keys, msgs)[key := msg]
+  ensures key !in BucketMapOfSeq(keys, msgs)
+  {
+    reveal_BucketMapOfSeq();
+    if key in BucketMapOfSeq(keys, msgs) {
+      var i := BucketMapOfSeqGetIndex(keys, msgs, key);
+      assert Keyspace.lt(keys[i], key);
+    }
+  }
+
+  lemma BucketMapOfSeqPopFront(
+      keys: seq<Key>, msgs: seq<Message>, i: int)
+  requires |keys| == |msgs|
+  requires 0 <= i < |keys|
+  requires IsStrictlySorted(keys)
+  ensures BucketMapOfSeq(keys[i+1..], msgs[i+1..])[keys[i] := msgs[i]]
+       == BucketMapOfSeq(keys[i..], msgs[i..])
+  ensures keys[i] !in BucketMapOfSeq(keys[i+1..], msgs[i+1..])
+  {
+    var a := BucketMapOfSeq(keys[i+1..], msgs[i+1..])[keys[i] := msgs[i]];
+    var b := BucketMapOfSeq(keys[i..], msgs[i..]);
+    forall k | k in a
+    ensures k in b
+    ensures a[k] == b[k]
+    {
+      reveal_IsStrictlySorted();
+      if k == keys[i] {
+        BucketMapOfSeqMapsIndex(keys[i..], msgs[i..], 0);
+        assert a[k] == b[k];
+      } else {
+        var j := BucketMapOfSeqGetIndex(keys[i+1..], msgs[i+1..], k);
+        BucketMapOfSeqMapsIndex(keys[i..], msgs[i..], j+1);
+        assert a[k] == b[k];
+      }
+    }
+    forall k | k in b
+    ensures k in a
+    {
+    }
+    reveal_IsStrictlySorted();
+  }
+
+  lemma flushedMapPopFront(res: singleMergeResult,
+    top_keys: seq<Key>, top_msgs: seq<Message>, from: int, to: int)
+  requires |top_keys| == |top_msgs|
+  requires 0 <= from < to <= |top_keys|
+  requires res.SlackExhausted? ==> from+1 <= res.end <= |top_keys|
+  requires IsStrictlySorted(top_keys)
+  ensures res.flushedMap(top_keys, top_msgs, from, to)
+      == res.flushedMap(top_keys, top_msgs, from+1, to)
+              [top_keys[from] := top_msgs[from]]
+  ensures top_keys[from] !in res.flushedMap(top_keys, top_msgs, from+1, to)
+  {
+    var a := BucketMapOfSeq(top_keys[from+1..to], top_msgs[from+1..to])[top_keys[from] := top_msgs[from]];
+    var b := BucketMapOfSeq(top_keys[from..to], top_msgs[from..to]);
+    forall k | k in a
+    ensures k in b
+    ensures a[k] == b[k]
+    {
+      reveal_IsStrictlySorted();
+      if k == top_keys[from] {
+        BucketMapOfSeqMapsIndex(top_keys[from..to], top_msgs[from..to], 0);
+        assert a[k] == b[k];
+      } else {
+        var j := BucketMapOfSeqGetIndex(top_keys[from+1..to], top_msgs[from+1..to], k);
+        BucketMapOfSeqMapsIndex(top_keys[from..to], top_msgs[from..to], j+1);
+        assert a[k] == b[k];
+      }
+    }
+    forall k | k in b
+    ensures k in a
+    {
+    }
+    assert BucketMapOfSeq(top_keys[from+1..to], top_msgs[from+1..to])[top_keys[from] := top_msgs[from]]
+        ==  BucketMapOfSeq(top_keys[from..to], top_msgs[from..to]);
+    reveal_IsStrictlySorted();
+  }
+
+  predicate seq_lt(a: seq<Key>, b: seq<Key>, start: int)
+  requires 0 <= start <= |b|
+  {
+    forall i, j | 0 <= i < |a| && start <= j < |b| ::
+      Keyspace.lt(a[i], b[j])
+  }
+
+  lemma topBotAccMerge_concat_lists(
+      acc_keys: seq<Key>, acc_msgs: seq<Message>,
+      bot_keys: seq<Key>, bot_msgs: seq<Message>,
+      from: int)
+  requires |acc_keys| == |acc_msgs|
+  requires |bot_keys| == |bot_msgs|
+  requires 0 <= from <= |bot_keys|
+  requires IsStrictlySorted(acc_keys)
+  requires IsStrictlySorted(bot_keys)
+  requires forall i | 0 <= i < |acc_msgs| :: acc_msgs[i] != IdentityMessage()
+  requires forall i | 0 <= i < |bot_msgs| :: bot_msgs[i] != IdentityMessage()
+  requires seq_lt(acc_keys, bot_keys, from)
+  ensures
+    topBotAccMerge(map[],
+      BucketMapOfSeq(bot_keys[from..], bot_msgs[from..]),
+      BucketMapOfSeq(acc_keys, acc_msgs))
+    == BucketMapOfSeq(acc_keys + bot_keys[from..], acc_msgs + bot_msgs[from..])
+  {
+    var x := 
+      topBotAccMerge(map[],
+        BucketMapOfSeq(bot_keys[from..], bot_msgs[from..]),
+        BucketMapOfSeq(acc_keys, acc_msgs));
+    var y := BucketMapOfSeq(acc_keys + bot_keys[from..], acc_msgs + bot_msgs[from..]);
+    forall k: Key | k in y
+    ensures k in x
+    ensures x[k] == y[k]
+    {
+      reveal_IsStrictlySorted();
+      var i := BucketMapOfSeqGetIndex(acc_keys + bot_keys[from..], acc_msgs + bot_msgs[from..], k);
+      if i < |acc_keys| {
+        BucketMapOfSeqMapsIndex(acc_keys, acc_msgs, i);
+        assert k !in BucketMapOfSeq(bot_keys[from..], bot_msgs[from..]);
+      } else {
+        BucketMapOfSeqMapsIndex(bot_keys[from..], bot_msgs[from..], i - |acc_keys|);
+        assert k !in BucketMapOfSeq(acc_keys, acc_msgs);
+      }
+    }
+    forall k | k in x
+    ensures k in y
+    {
+    }
+  }
+
+  lemma mergeToOneOneChild_eq_topBotAccMerge(
+      top_keys: seq<Key>,
+      top_msgs: seq<Message>,
+      from: nat,
+      to: nat,
+      bot_keys: seq<Key>,
+      bot_msgs: seq<Message>,
+      bot_from: nat,
+      acc_keys: seq<Key>,
+      acc_msgs: seq<Message>,
+      slack: nat)
+  requires |top_keys| == |top_msgs|
+  requires |bot_keys| == |bot_msgs|
+  requires |acc_keys| == |acc_msgs|
+  requires from <= to <= |top_keys|
+  requires bot_from <= |bot_keys|
+  requires IsStrictlySorted(acc_keys)
+  requires IsStrictlySorted(top_keys)
+  requires IsStrictlySorted(bot_keys)
+  requires seq_lt(acc_keys, top_keys, from)
+  requires seq_lt(acc_keys, bot_keys, bot_from)
+  requires forall i | 0 <= i < |bot_msgs| :: bot_msgs[i] != IdentityMessage()
+  requires forall i | 0 <= i < |top_msgs| :: top_msgs[i] != IdentityMessage()
+  requires forall i | 0 <= i < |acc_msgs| :: acc_msgs[i] != IdentityMessage()
+  decreases |top_keys| + |bot_keys| - from - bot_from
+  ensures
+      var res := mergeToOneChild(
+            top_keys, top_msgs, from, to,
+            bot_keys, bot_msgs, bot_from,
+            acc_keys, acc_msgs, slack);
+      var top := BucketMapOfSeq(
+            top_keys[from..to], top_msgs[from..to]);
+      var bot := BucketMapOfSeq(
+            bot_keys[bot_from..], bot_msgs[bot_from..]);
+      var acc := BucketMapOfSeq(acc_keys, acc_msgs);
+      res.bucketMap() == topBotAccMerge(
+        res.flushedMap(top_keys, top_msgs, from, to),
+        bot, acc)
+  {
+    var res := mergeToOneChild(
+          top_keys, top_msgs, from, to,
+          bot_keys, bot_msgs, bot_from,
+          acc_keys, acc_msgs, slack);
+    var top := BucketMapOfSeq(
+          top_keys[from..to], top_msgs[from..to]);
+    var bot := BucketMapOfSeq(
+          bot_keys[bot_from..], bot_msgs[bot_from..]);
+    var acc := BucketMapOfSeq(acc_keys, acc_msgs);
+
+    assert IsStrictlySorted(bot_keys[bot_from..]) by { reveal_IsStrictlySorted(); }
+    assert IsStrictlySorted(top_keys[from..to]) by { reveal_IsStrictlySorted(); }
+
+    if from == to {
+      var a := res.bucketMap();
+      var b := topBotAccMerge(
+        res.flushedMap(top_keys, top_msgs, from, to),
+        bot, acc);
+      forall k | k in a
+      ensures k in b
+      ensures a[k] == b[k]
+      {
+        var i := BucketMapOfSeqGetIndex(res.keys, res.msgs, k);
+        if i < |acc_keys| {
+          BucketMapOfSeqMapsIndex(acc_keys, acc_msgs, i);
+        } else {
+          BucketMapOfSeqMapsIndex(bot_keys[bot_from..],
+              bot_msgs[bot_from..], i-|acc_keys|);
+        }
+      }
+      forall k | k in b
+      ensures k in a
+      {
+      }
+      assert a == b;
+    } else if |bot_keys| == bot_from {
+      var a := res.bucketMap();
+      var b := topBotAccMerge(
+        res.flushedMap(top_keys, top_msgs, from, to),
+        bot, acc);
+      forall k | k in a
+      ensures k in b
+      ensures a[k] == b[k]
+      {
+        var i := BucketMapOfSeqGetIndex(res.keys, res.msgs, k);
+        if i < |acc_keys| {
+          BucketMapOfSeqMapsIndex(acc_keys, acc_msgs, i);
+          /*assert acc_msgs[i] != IdentityMessage();
+          assert k !in bot;
+          assert k !in top;
+          assert k !in res.flushedMap(top_keys, top_msgs, from, to);
+          assert k in acc;
+          assert k in acc.Keys;
+          assert topBotAccMergeForKey(
+            res.flushedMap(top_keys, top_msgs, from, to),
+            bot, acc, k)
+              == acc_msgs[i];
+          assert topBotAccMergeForKey(
+            res.flushedMap(top_keys, top_msgs, from, to),
+            bot, acc, k) != IdentityMessage();*/
+          assert k in b;
+        } else {
+          BucketMapOfSeqMapsIndex(top_keys[from..to], top_msgs[from..to], i - |acc_keys|);
+          assert k in res.flushedMap(top_keys, top_msgs, from, to);
+          assert k in b;
+        }
+      }
+      forall k | k in b
+      ensures k in a
+      {
+      }
+      assert a == b;
+    } else if top_keys[from] == bot_keys[bot_from] {
+      var key := top_keys[from];
+      var topmsg := top_msgs[from];
+      var botmsg := bot_msgs[bot_from];
+      var msg := ValueMessage.Merge(topmsg, botmsg);
+      if msg == IdentityMessage() {
+        calc {
+          res.bucketMap();
+          {
+            mergeToOneOneChild_eq_topBotAccMerge(
+                top_keys, top_msgs, from+1, to,
+                bot_keys, bot_msgs, bot_from+1,
+                acc_keys, acc_msgs,
+                slack + WeightKey(key) + WeightMessage(botmsg));
+          }
+          topBotAccMerge(
+            res.flushedMap(top_keys, top_msgs, from+1, to),
+            BucketMapOfSeq(bot_keys[bot_from+1..], bot_msgs[bot_from+1..]),
+            BucketMapOfSeq(acc_keys, acc_msgs));
+          {
+            flushedMapPopFront(res, top_keys, top_msgs, from, to);
+            assert res.flushedMap(top_keys, top_msgs, from, to)
+                == res.flushedMap(top_keys, top_msgs, from+1, to)[key := topmsg];
+            BucketMapOfSeqPopFront(bot_keys, bot_msgs, bot_from);
+            assert BucketMapOfSeq(bot_keys[bot_from..], bot_msgs[bot_from..])
+                == BucketMapOfSeq(bot_keys[bot_from+1..], bot_msgs[bot_from+1..])[key := botmsg];
+            assert key !in acc;
+            assert key !in BucketMapOfSeq(bot_keys[bot_from+1..], bot_msgs[bot_from+1..]);
+            assert key !in res.flushedMap(top_keys, top_msgs, from+1, to);
+          }
+          topBotAccMerge(
+            res.flushedMap(top_keys, top_msgs, from, to),
+            bot, acc);
+        }
+      } else {
+        var delta := WeightMessage(msg) - WeightMessage(botmsg);
+        if delta > slack {
+          calc {
+            res.bucketMap();
+            {
+              assert res.flushedMap(top_keys, top_msgs, from, to)
+                  == map[];
+              topBotAccMerge_concat_lists(acc_keys, acc_msgs, bot_keys, bot_msgs, bot_from);
+            }
+            topBotAccMerge(
+              res.flushedMap(top_keys, top_msgs, from, to),
+              bot, acc);
+          }
+        } else {
+          calc {
+            res.bucketMap();
+            {
+              reveal_IsStrictlySorted();
+              mergeToOneOneChild_eq_topBotAccMerge(
+                  top_keys, top_msgs, from+1, to,
+                  bot_keys, bot_msgs, bot_from+1,
+                  acc_keys + [key], acc_msgs + [msg],
+                  slack - delta);
+            }
+            topBotAccMerge(
+              res.flushedMap(top_keys, top_msgs, from+1, to),
+              BucketMapOfSeq(
+                  bot_keys[bot_from+1..], bot_msgs[bot_from+1..]),
+              BucketMapOfSeq(acc_keys + [key], acc_msgs + [msg])
+            );
+            {
+              BucketMapOfSeqPushBack(acc_keys, acc_msgs, key, msg);
+              flushedMapPopFront(res, top_keys, top_msgs, from, to);
+              BucketMapOfSeqPopFront(bot_keys, bot_msgs, bot_from);
+            }
+            topBotAccMerge(
+              res.flushedMap(top_keys, top_msgs, from, to),
+              bot, acc);
+          }
+        }
+      }
+    } else if Keyspace.lt(top_keys[from], bot_keys[bot_from]) {
+      var key := top_keys[from];
+      var msg := top_msgs[from];
+      var delta := WeightKey(key) + WeightMessage(msg);
+      if delta > slack {
+        calc {
+          res.bucketMap();
+          {
+            assert res.flushedMap(top_keys, top_msgs, from, to)
+                == map[];
+            topBotAccMerge_concat_lists(acc_keys, acc_msgs, bot_keys, bot_msgs, bot_from);
+          }
+          topBotAccMerge(
+            res.flushedMap(top_keys, top_msgs, from, to),
+            bot, acc);
+        }
+      } else {
+        calc {
+          res.bucketMap();
+          {
+            //StrictlySortedAugment(acc_keys, key);
+            reveal_IsStrictlySorted();
+            mergeToOneOneChild_eq_topBotAccMerge(
+                top_keys, top_msgs, from+1, to,
+                bot_keys, bot_msgs, bot_from,
+                acc_keys + [key], acc_msgs + [msg],
+                slack - delta);
+          }
+          topBotAccMerge(
+            res.flushedMap(top_keys, top_msgs, from+1, to),
+            bot, BucketMapOfSeq(acc_keys + [key], acc_msgs + [msg]));
+          {
+            BucketMapOfSeqPushBack(acc_keys, acc_msgs, key, msg);
+            flushedMapPopFront(res, top_keys, top_msgs, from, to);
+          }
+          topBotAccMerge(
+            res.flushedMap(top_keys, top_msgs, from, to),
+            bot, acc);
+        }
+      }
+    } else {
+      var key := bot_keys[bot_from];
+      var msg := bot_msgs[bot_from];
+
+      calc {
+        res.bucketMap();
+        {
+          reveal_IsStrictlySorted();
+          mergeToOneOneChild_eq_topBotAccMerge(
+              top_keys, top_msgs, from, to,
+              bot_keys, bot_msgs, bot_from+1,
+              acc_keys + [key], acc_msgs + [msg],
+              slack);
+        }
+        topBotAccMerge(
+          res.flushedMap(top_keys, top_msgs, from, to),
+          BucketMapOfSeq(
+              bot_keys[bot_from+1..], bot_msgs[bot_from+1..]),
+          BucketMapOfSeq(acc_keys + [key], acc_msgs + [msg]));
+        {
+          BucketMapOfSeqPopFront(bot_keys, bot_msgs, bot_from);
+          BucketMapOfSeqPushBack(acc_keys, acc_msgs, key, msg);
+        }
+        topBotAccMerge(
+          res.flushedMap(top_keys, top_msgs, from, to),
+          bot,
+          acc);
+      }
+    }
+  }
+
+  function bucketStartIdx(top_keys: seq<Key>, pivots: PivotTable, r: int) : int
+  requires 0 <= r <= |pivots|
+  {
+    if r == 0 then 0 else binarySearchIndexOfFirstKeyGte(top_keys, pivots[r-1])
+  }
+
+  function bucketEndIdx(top_keys: seq<Key>, pivots: PivotTable, r: int) : int
+  requires 0 <= r <= |pivots|
+  {
+    if r < |pivots| then binarySearchIndexOfFirstKeyGte(top_keys, pivots[r]) else |top_keys|
+  }
+
+  lemma mergeToOneOneChild_eq_BucketList(
+      top_keys: seq<Key>,
+      top_msgs: seq<Message>,
+      from: nat,
+      to: nat,
+      bot_keys: seq<Key>,
+      bot_msgs: seq<Message>,
+      slack: nat,
+      pivots: PivotTable,
+      r: int)
+  requires |top_keys| == |top_msgs|
+  requires |bot_keys| == |bot_msgs|
+  requires from <= to <= |top_keys|
+  requires 0 <= r <= |pivots|
+  requires from == bucketStartIdx(top_keys, pivots, r)
+  requires to == bucketStartIdx(top_keys, pivots, r)
+  requires IsStrictlySorted(top_keys)
+  requires IsStrictlySorted(bot_keys)
+  requires forall i | 0 <= i < |bot_msgs| :: bot_msgs[i] != IdentityMessage()
+  requires forall i | 0 <= i < |top_msgs| :: top_msgs[i] != IdentityMessage()
+  requires WFPivots(pivots)
+  requires forall i | 0 <= i < |bot_keys| :: Route(pivots, bot_keys[i]) == r
+  ensures
+      var res := mergeToOneChild(
+            top_keys, top_msgs, from, to,
+            bot_keys, bot_msgs, 0,
+            [], [], slack);
+      var top := BucketMapOfSeq(top_keys, top_msgs);
+      var bot := BucketMapOfSeq(bot_keys, bot_msgs);
+      BucketListItemFlush(
+          BucketIntersect(B(top), res.flushedKeys(top_keys, top_msgs, from, to)),
+          B(bot), pivots, r).b
+        == res.bucketMap()
+  {
+
+    var res := mergeToOneChild(
+          top_keys, top_msgs, from, to,
+          bot_keys, bot_msgs, 0,
+          [], [], slack);
+    var top := BucketMapOfSeq(top_keys, top_msgs);
+    var bot := BucketMapOfSeq(bot_keys, bot_msgs);
+
+    var itop := BucketIntersect(B(top), res.flushedKeys(top_keys, top_msgs, from, to));
+
+    calc {
+      BucketListItemFlush(itop, B(bot), pivots, r).b;
+      {
+        var a := BucketListItemFlush(itop, B(bot), pivots, r).b;
+        var b := topBotAccMerge(itop.b, bot, map[]);
+        forall k | k in a
+        ensures k in b
+        ensures a[k] == b[k]
+        {
+        }
+        forall k | k in b
+        ensures k in a
+        {
+          reveal_BucketIntersect();
+          RouteIs(pivots, k, r);
+        }
+      }
+      topBotAccMerge(itop.b, bot, map[]);
+      topBotAccMerge(
+        itop.b,
+        BucketMapOfSeq(bot_keys, bot_msgs),
+        map[]);
+      {
+        reveal_BucketIntersect();
+        assert itop.b == res.flushedMap(top_keys, top_msgs, from, to);
+      }
+      topBotAccMerge(
+        res.flushedMap(top_keys, top_msgs, from, to),
+        BucketMapOfSeq(bot_keys, bot_msgs),
+        map[]);
+      topBotAccMerge(
+        res.flushedMap(top_keys, top_msgs, from, to),
+        BucketMapOfSeq(bot_keys, bot_msgs),
+        BucketMapOfSeq([], []));
+      {
+        mergeToOneOneChild_eq_topBotAccMerge(
+          top_keys, top_msgs, from, to, bot_keys, bot_msgs, 0,
+          [], [], slack);
+      }
+      res.bucketMap();
+    }
+  }
+
+  function pivotIndexes(top_keys: seq<Key>, pivots: seq<Key>) : (res: seq<int>)
+  ensures |res| == |pivots|
+  ensures forall i | 0 <= i < |res| :: res[i]
+      == binarySearchIndexOfFirstKeyGte(top_keys, pivots[i])
+  {
+    if |pivots| == 0 then (
+      []
+    ) else (
+      pivotIndexes(top_keys, DropLast(pivots)) +
+        [binarySearchIndexOfFirstKeyGte(top_keys, Last(pivots))]
+    )
+  }
+
+  datatype mergeResult = mergeResult(
+    top: Bucket,
+    bots: seq<Bucket>,
+    slack: nat)
+
+  function mergeToChildrenIter(
+      top: Bucket,
+      pivots: seq<Key>,
+      bots: seq<Bucket>,
+      idxs: seq<int>,
+      tmp: singleMergeResult,
+      i: int,
+      results: seq<Bucket>) : (res : mergeResult)
+  requires WFBucket(top)
+  requires forall i | 0 <= i < |bots| :: WFBucket(bots[i])
+  requires 0 < |bots| == |pivots| + 1
+  requires |results| == i
+  requires |idxs| == |pivots|
+  requires 0 <= i <= |bots|
+  requires forall i | 0 <= i < |idxs| :: 0 <= idxs[i] <= |top.keys|
+  requires tmp.SlackExhausted? ==> 0 <= tmp.end <= |top.keys|
+  decreases |bots| - i
+  ensures |res.bots| == |bots|
+  {
+    if i == |bots| then (
+      if tmp.SlackExhausted? then (
+        var leftover_top := B(BucketMapOfSeq(top.keys[tmp.end..], top.msgs[tmp.end..]));
+        mergeResult(leftover_top, results, tmp.slack)
+      ) else (
+        mergeResult(B(map[]), results, tmp.slack)
+      )
+    ) else (
+      if tmp.MergeCompleted? then (
+        var from := if i == 0 then 0 else idxs[i-1];
+        var to1 := if i == |idxs| then |top.keys| else idxs[i];
+        var to := if to1 < from then from else to1;
+        var tmp' := mergeToOneChild(
+            top.keys, top.msgs, from, to,
+            bots[i].keys, bots[i].msgs, 0,
+            [], [], tmp.slack);
+        var results' := results + [B(tmp'.bucketMap())];
+        mergeToChildrenIter(top, pivots, bots, idxs, tmp', i+1, results')
+      ) else (
+        var results' := results + [bots[i]];
+        mergeToChildrenIter(top, pivots, bots, idxs, tmp, i+1, results')
+      )
+    )
+  }
+ 
+  function mergeToChildren(
+      top: Bucket,
+      pivots: seq<Key>,
+      bots: seq<Bucket>,
+      slack: nat) : (result: mergeResult)
+  requires WFBucket(top)
+  requires forall i | 0 <= i < |bots| :: WFBucket(bots[i])
+  requires 0 < |bots| == |pivots| + 1
+  {
+    var idxs := pivotIndexes(top.keys, pivots);
+    var tmp := MergeCompleted([], [], slack);
+    mergeToChildrenIter(top, pivots, bots, idxs, tmp, 0, [])
+  }
+
 }
